updates

Veritas.EAC.fst
@@ -147,7 +147,17 @@ let last_put_value_or_null (l:vlog) =
   if has_some_put l then Put?.v (index l (last_put_idx l))
   else Null
 
-//let lemma_eac_add_closure (st: eac_state {EACFail st ||
+let eac_closure_pred1 (st: eac_state): bool =
+  EACFail = st ||  valid_eac_state st && DVal? (value_of st)
+
+let eac_closure_pred2 (st: eac_state): bool =
+  EACFail = st ||  valid_eac_state st && MVal? (value_of st)
+
+let lemma_eac_add_closure1 (e:vlog_entry_ext) (st: eac_state):
+  Lemma (eac_closure_pred1 st ==> eac_closure_pred1 (eac_add e st)) = ()
+
+let lemma_eac_add_closure2 (e:vlog_entry_ext) (st: eac_state):
+  Lemma (eac_closure_pred2 st ==> eac_closure_pred2 (eac_add e st)) = ()
 
 let lemma_value_type (le:vlog_ext {length le > 0}):
   Lemma (EACFail = seq_machine_run eac_smk le \/
@@ -156,7 +166,26 @@ let lemma_value_type (le:vlog_ext {length le > 0}):
          DVal? (value_of (seq_machine_run eac_smk le)) =
          DVal? (value_of (seq_machine_run eac_smk (prefix le 1)))) =
 
-  admit()
+  let n = length le in
+  let st = seq_machine_run eac_smk le in
+
+  if EACFail = st then ()
+
+  else (
+    // st1 is valid (and not init)
+    lemma_valid_prefix eac_smk le 1;
+    lemma_notempty_implies_noninit eac_smk (prefix le 1);
+    let st1 = seq_machine_run eac_smk (prefix le 1) in
+    assert(valid_eac_state st1);
+
+    lemma_reduce_prefix EACInit eac_add le 1;
+    assert(st = reduce st1 eac_add (suffix le (n - 1)));
+
+    if DVal? (value_of st1) then
+      lemma_reduce_property_closure eac_closure_pred1 st1 eac_add (suffix le (n - 1))
+    else
+      lemma_reduce_property_closure eac_closure_pred2 st1 eac_add (suffix le (n - 1))
+  )
 
 let lemma_first_entry_is_madd (le:vlog_ext):
   Lemma (requires (valid eac_smk le /\ length le > 0))
